chore: cleanup for presentation

tests/lean/run/letrecInProofs.lean
@@ -4,22 +4,24 @@ inductive Tree
   | leaf : Tree
   | node : Tree → Tree → Tree
 
-abbrev notLtX (x : Tree) (t : Tree) : Prop :=
+abbrev notSubtree (x : Tree) (t : Tree) : Prop :=
   Tree.ibelow (motive := fun z => x ≠ z) t
 
-theorem Tree.acyclic (x t : Tree) : x = t → notLtX x t := by
-  let rec right (x s : Tree) (b : Tree) (h : notLtX x b) : node s x ≠ b ∧ notLtX (node s x) b := by
+infix:50 "≮" => notSubtree
+
+theorem Tree.acyclic (x t : Tree) : x = t → x ≮ t := by
+  let rec right (x s : Tree) (b : Tree) (h : x ≮ b) : node s x ≠ b ∧ node s x ≮ b := by
     match b, h with
     | leaf,     h =>
       apply And.intro _ trivial
       intro h; injection h
     | node l r, h =>
-      have ihl : notLtX x l → node s x ≠ l ∧ notLtX (node s x) l from right x s l
-      have ihr : notLtX x r → node s x ≠ r ∧ notLtX (node s x) r from right x s r
-      have hl : x ≠ l ∧ notLtX x l from h.1
-      have hr : x ≠ r ∧ notLtX x r from h.2.1
-      have ihl : node s x ≠ l ∧ notLtX (node s x) l from ihl hl.2
-      have ihr : node s x ≠ r ∧ notLtX (node s x) r from ihr hr.2
+      have ihl : x ≮ l → node s x ≠ l ∧ node s x ≮ l from right x s l
+      have ihr : x ≮ r → node s x ≠ r ∧ node s x ≮ r from right x s r
+      have hl : x ≠ l ∧ x ≮ l from h.1
+      have hr : x ≠ r ∧ x ≮ r from h.2.1
+      have ihl : node s x ≠ l ∧ node s x ≮ l from ihl hl.2
+      have ihr : node s x ≠ r ∧ node s x ≮ r from ihr hr.2
       apply And.intro
       focus
         intro h
@@ -31,18 +33,18 @@ theorem Tree.acyclic (x t : Tree) : x = t → notLtX x t := by
         apply ihl
         apply And.intro _ trivial
         apply ihr
-  let rec left (x t : Tree) (b : Tree) (h : notLtX x b) : node x t ≠ b ∧ notLtX (node x t) b := by
+  let rec left (x t : Tree) (b : Tree) (h : x ≮ b) : node x t ≠ b ∧ node x t ≮ b := by
     match b, h with
     | leaf, h     =>
       apply And.intro _ trivial
       intro h; injection h
     | node l r, h =>
-      have ihl : notLtX x l → node x t ≠ l ∧ notLtX (node x t) l from left x t l
-      have ihr : notLtX x r → node x t ≠ r ∧ notLtX (node x t) r from left x t r
-      have hl : x ≠ l ∧ notLtX x l from h.1
-      have hr : x ≠ r ∧ notLtX x r from h.2.1
-      have ihl : node x t ≠ l ∧ notLtX (node x t) l from ihl hl.2
-      have ihr : node x t ≠ r ∧ notLtX (node x t) r from ihr hr.2
+      have ihl : x ≮ l → node x t ≠ l ∧ node x t ≮ l from left x t l
+      have ihr : x ≮ r → node x t ≠ r ∧ node x t ≮ r from left x t r
+      have hl : x ≠ l ∧ x ≮ l from h.1
+      have hr : x ≠ r ∧ x ≮ r from h.2.1
+      have ihl : node x t ≠ l ∧ node x t ≮ l from ihl hl.2
+      have ihr : node x t ≠ r ∧ node x t ≮ r from ihr hr.2
       apply And.intro
       focus
         intro h
@@ -54,12 +56,12 @@ theorem Tree.acyclic (x t : Tree) : x = t → notLtX x t := by
         apply ihl
         apply And.intro _ trivial
         apply ihr
-  let rec aux : (x : Tree) → notLtX x x
+  let rec aux : (x : Tree) → x ≮ x
     | leaf     => trivial
     | node l r => by
-        have ih₁ : notLtX l l from aux l
-        have ih₂ : notLtX r r from aux r
-        show (node l r ≠ l ∧ notLtX (node l r) l) ∧ (node l r ≠ r ∧ notLtX (node l r) r) ∧ True
+        have ih₁ : l ≮ l from aux l
+        have ih₂ : r ≮ r from aux r
+        show (node l r ≠ l ∧ node l r ≮ l) ∧ (node l r ≠ r ∧ node l r ≮ r) ∧ True
         apply And.intro
         focus
           apply left
